programs/lean/Project/ReverseInplace/Program.lean
@@ -80,6 +80,9 @@ def func0 : Wasm.Program :=
   .unreachable
 ]
 
+def func0Def : Wasm.Function :=
+  { params := [.i32, .i32], locals := [.i32, .i32, .i32, .i32], body := func0, results := [] }
+
 def func1 : Wasm.Program :=
   [
   .globalGet 0,
@@ -146,6 +149,9 @@ def func1 : Wasm.Program :=
     ]
   ]
 ]
+
+def func1Def : Wasm.Function :=
+  { params := [.i32, .i32], locals := [.i32, .i32, .i32, .i32], body := func1, results := [] }
 
 def func2 : Wasm.Program :=
   [
@@ -274,6 +280,9 @@ def func2 : Wasm.Program :=
   .globalSet 0
 ]
 
+def func2Def : Wasm.Function :=
+  { params := [.i32, .i32], locals := [.i32, .i32, .i32, .i32], body := func2, results := [] }
+
 /-- export: check -/
 def func3 : Wasm.Program :=
   [
@@ -281,6 +290,9 @@ def func3 : Wasm.Program :=
   .localGet 1,
   .call 2
 ]
+
+def func3Def : Wasm.Function :=
+  { params := [.i32, .i32], locals := [], body := func3, results := [] }
 
 def func4 : Wasm.Program :=
   [
@@ -290,6 +302,9 @@ def func4 : Wasm.Program :=
   .ret
 ]
 
+def func4Def : Wasm.Function :=
+  { params := [.i32, .i32], locals := [], body := func4, results := [.i32] }
+
 def func5 : Wasm.Program :=
   [
   .localGet 0,
@@ -298,6 +313,9 @@ def func5 : Wasm.Program :=
   .call 25,
   .ret
 ]
+
+def func5Def : Wasm.Function :=
+  { params := [.i32, .i32, .i32], locals := [], body := func5, results := [] }
 
 def func6 : Wasm.Program :=
   [
@@ -309,16 +327,25 @@ def func6 : Wasm.Program :=
   .ret
 ]
 
+def func6Def : Wasm.Function :=
+  { params := [.i32, .i32, .i32, .i32], locals := [], body := func6, results := [.i32] }
+
 def func7 : Wasm.Program :=
   [
   .ret
 ]
+
+def func7Def : Wasm.Function :=
+  { params := [], locals := [], body := func7, results := [] }
 
 def func8 : Wasm.Program :=
   [
   .call 24,
   .unreachable
 ]
+
+def func8Def : Wasm.Function :=
+  { params := [.i32, .i32], locals := [], body := func8, results := [.i32] }
 
 def func9 : Wasm.Program :=
   [
@@ -408,6 +435,9 @@ def func9 : Wasm.Program :=
   .globalSet 0
 ]
 
+def func9Def : Wasm.Function :=
+  { params := [.i32, .i32, .i32, .i32, .i32], locals := [.i32], body := func9, results := [] }
+
 def func10 : Wasm.Program :=
   [
   .block 0 0 [
@@ -423,6 +453,9 @@ def func10 : Wasm.Program :=
     .call 5
   ]
 ]
+
+def func10Def : Wasm.Function :=
+  { params := [.i32, .i32], locals := [], body := func10, results := [] }
 
 def func11 : Wasm.Program :=
   [
@@ -440,6 +473,9 @@ def func11 : Wasm.Program :=
     .call 5
   ]
 ]
+
+def func11Def : Wasm.Function :=
+  { params := [.i32], locals := [.i32], body := func11, results := [] }
 
 def func12 : Wasm.Program :=
   [
@@ -459,12 +495,18 @@ def func12 : Wasm.Program :=
   ]
 ]
 
+def func12Def : Wasm.Function :=
+  { params := [.i32], locals := [.i32], body := func12, results := [] }
+
 def func13 : Wasm.Program :=
   [
   .localGet 0,
   .call 14,
   .unreachable
 ]
+
+def func13Def : Wasm.Function :=
+  { params := [.i32], locals := [], body := func13, results := [] }
 
 def func14 : Wasm.Program :=
   [
@@ -483,12 +525,18 @@ def func14 : Wasm.Program :=
   .unreachable
 ]
 
+def func14Def : Wasm.Function :=
+  { params := [.i32], locals := [], body := func14, results := [] }
+
 def func15 : Wasm.Program :=
   [
   .localGet 0,
   .call 16,
   .unreachable
 ]
+
+def func15Def : Wasm.Function :=
+  { params := [.i32], locals := [], body := func15, results := [] }
 
 def func16 : Wasm.Program :=
   [
@@ -555,6 +603,9 @@ def func16 : Wasm.Program :=
   .call 18,
   .unreachable
 ]
+
+def func16Def : Wasm.Function :=
+  { params := [.i32], locals := [.i32, .i32, .i32], body := func16, results := [] }
 
 def func17 : Wasm.Program :=
   [
@@ -649,6 +700,9 @@ def func17 : Wasm.Program :=
   .localGet 6,
   .store32 (0 : UInt32)
 ]
+
+def func17Def : Wasm.Function :=
+  { params := [.i32, .i32, .i32, .i32, .i32, .i32], locals := [.i32, .i32, .i64], body := func17, results := [] }
 
 def func18 : Wasm.Program :=
   [
@@ -747,12 +801,18 @@ def func18 : Wasm.Program :=
   .unreachable
 ]
 
+def func18Def : Wasm.Function :=
+  { params := [.i32, .i32, .i32, .i32, .i32], locals := [.i32, .i32], body := func18, results := [] }
+
 def func19 : Wasm.Program :=
   [
   .const (0 : UInt32),
   .const (1 : UInt32),
   .store8 (1049788 : UInt32)
 ]
+
+def func19Def : Wasm.Function :=
+  { params := [.i32, .i32], locals := [], body := func19, results := [] }
 
 def func20 : Wasm.Program :=
   [
@@ -762,6 +822,9 @@ def func20 : Wasm.Program :=
   .drop,
   .unreachable
 ]
+
+def func20Def : Wasm.Function :=
+  { params := [.i32, .i32], locals := [], body := func20, results := [] }
 
 def func21 : Wasm.Program :=
   [
@@ -778,6 +841,9 @@ def func21 : Wasm.Program :=
   .localGet 0,
   .call 23
 ]
+
+def func21Def : Wasm.Function :=
+  { params := [.i32, .i32], locals := [], body := func21, results := [.i32] }
 
 def func22 : Wasm.Program :=
   [
@@ -999,6 +1065,9 @@ def func22 : Wasm.Program :=
   ],
   .localGet 2
 ]
+
+def func22Def : Wasm.Function :=
+  { params := [.i32, .i32], locals := [.i32, .i32, .i32, .i32, .i32], body := func22, results := [.i32] }
 
 def func23 : Wasm.Program :=
   [
@@ -3250,10 +3319,16 @@ def func23 : Wasm.Program :=
   .localGet 0
 ]
 
+def func23Def : Wasm.Function :=
+  { params := [.i32], locals := [.i32, .i32, .i32, .i32, .i32, .i32, .i32, .i32, .i32, .i64], body := func23, results := [.i32] }
+
 def func24 : Wasm.Program :=
   [
   .unreachable
 ]
+
+def func24Def : Wasm.Function :=
+  { params := [], locals := [], body := func24, results := [] }
 
 def func25 : Wasm.Program :=
   [
@@ -3308,6 +3383,9 @@ def func25 : Wasm.Program :=
   .call 52,
   .unreachable
 ]
+
+def func25Def : Wasm.Function :=
+  { params := [.i32, .i32, .i32], locals := [.i32, .i32], body := func25, results := [] }
 
 def func26 : Wasm.Program :=
   [
@@ -3709,6 +3787,9 @@ def func26 : Wasm.Program :=
     .store32 (1049776 : UInt32)
   ]
 ]
+
+def func26Def : Wasm.Function :=
+  { params := [.i32], locals := [.i32, .i32, .i32, .i32], body := func26, results := [] }
 
 def func27 : Wasm.Program :=
   [
@@ -4203,6 +4284,9 @@ def func27 : Wasm.Program :=
   .localGet 2
 ]
 
+def func27Def : Wasm.Function :=
+  { params := [.i32, .i32, .i32, .i32], locals := [.i32, .i32, .i32, .i32, .i32, .i32], body := func27, results := [.i32] }
+
 def func28 : Wasm.Program :=
   [
   .localGet 0,
@@ -4410,6 +4494,9 @@ def func28 : Wasm.Program :=
   .and,
   .store32 (1049748 : UInt32)
 ]
+
+def func28Def : Wasm.Function :=
+  { params := [.i32, .i32], locals := [.i32, .i32, .i32, .i32], body := func28, results := [] }
 
 def func29 : Wasm.Program :=
   [
@@ -4668,6 +4755,9 @@ def func29 : Wasm.Program :=
   ]
 ]
 
+def func29Def : Wasm.Function :=
+  { params := [.i32, .i32], locals := [.i32, .i32], body := func29, results := [] }
+
 def func30 : Wasm.Program :=
   [
   .globalGet 0,
@@ -4692,6 +4782,9 @@ def func30 : Wasm.Program :=
   .unreachable
 ]
 
+def func30Def : Wasm.Function :=
+  { params := [.i32], locals := [.i32, .i64], body := func30, results := [] }
+
 def func31 : Wasm.Program :=
   [
   .localGet 1,
@@ -4699,6 +4792,9 @@ def func31 : Wasm.Program :=
   .call 32,
   .unreachable
 ]
+
+def func31Def : Wasm.Function :=
+  { params := [.i32, .i32], locals := [], body := func31, results := [] }
 
 def func32 : Wasm.Program :=
   [
@@ -4720,6 +4816,9 @@ def func32 : Wasm.Program :=
   .call 13,
   .unreachable
 ]
+
+def func32Def : Wasm.Function :=
+  { params := [.i32, .i32], locals := [.i32], body := func32, results := [] }
 
 def func33 : Wasm.Program :=
   [
@@ -4895,6 +4994,9 @@ def func33 : Wasm.Program :=
   .store32 (8 : UInt32)
 ]
 
+def func33Def : Wasm.Function :=
+  { params := [.i32, .i32], locals := [.i32, .i32, .i32, .i32], body := func33, results := [] }
+
 def func34 : Wasm.Program :=
   [
   .const (0 : UInt32),
@@ -4932,6 +5034,9 @@ def func34 : Wasm.Program :=
   .localGet 1
 ]
 
+def func34Def : Wasm.Function :=
+  { params := [.i32], locals := [.i32, .i32], body := func34, results := [.i32] }
+
 def func35 : Wasm.Program :=
   [
   .localGet 0,
@@ -4944,6 +5049,9 @@ def func35 : Wasm.Program :=
   .store64 (0 : UInt32)
 ]
 
+def func35Def : Wasm.Function :=
+  { params := [.i32, .i32], locals := [], body := func35, results := [] }
+
 def func36 : Wasm.Program :=
   [
   .localGet 0,
@@ -4955,6 +5063,9 @@ def func36 : Wasm.Program :=
   .load64 (1048880 : UInt32),
   .store64 (0 : UInt32)
 ]
+
+def func36Def : Wasm.Function :=
+  { params := [.i32, .i32], locals := [], body := func36, results := [] }
 
 def func37 : Wasm.Program :=
   [
@@ -4987,6 +5098,9 @@ def func37 : Wasm.Program :=
   .call 54
 ]
 
+def func37Def : Wasm.Function :=
+  { params := [.i32, .i32], locals := [], body := func37, results := [.i32] }
+
 def func38 : Wasm.Program :=
   [
   .localGet 0,
@@ -4997,6 +5111,9 @@ def func38 : Wasm.Program :=
   .store32 (0 : UInt32)
 ]
 
+def func38Def : Wasm.Function :=
+  { params := [.i32, .i32], locals := [], body := func38, results := [] }
+
 def func39 : Wasm.Program :=
   [
   .localGet 0,
@@ -5004,6 +5121,9 @@ def func39 : Wasm.Program :=
   .load64 (0 : UInt32),
   .store64 (0 : UInt32)
 ]
+
+def func39Def : Wasm.Function :=
+  { params := [.i32, .i32], locals := [], body := func39, results := [] }
 
 def func40 : Wasm.Program :=
   [
@@ -5040,6 +5160,9 @@ def func40 : Wasm.Program :=
   .store32 (0 : UInt32)
 ]
 
+def func40Def : Wasm.Function :=
+  { params := [.i32, .i32], locals := [.i32, .i32], body := func40, results := [] }
+
 def func41 : Wasm.Program :=
   [
   .localGet 1,
@@ -5049,6 +5172,9 @@ def func41 : Wasm.Program :=
   .load32 (4 : UInt32),
   .call 59
 ]
+
+def func41Def : Wasm.Function :=
+  { params := [.i32, .i32], locals := [], body := func41, results := [.i32] }
 
 def func42 : Wasm.Program :=
   [
@@ -5200,6 +5326,9 @@ def func42 : Wasm.Program :=
   .const (0 : UInt32)
 ]
 
+def func42Def : Wasm.Function :=
+  { params := [.i32, .i32], locals := [.i32, .i32, .i32, .i32, .i32, .i32], body := func42, results := [.i32] }
+
 def func43 : Wasm.Program :=
   [
   .block 0 0 [
@@ -5248,6 +5377,9 @@ def func43 : Wasm.Program :=
   .store32 (8 : UInt32),
   .const (0 : UInt32)
 ]
+
+def func43Def : Wasm.Function :=
+  { params := [.i32, .i32, .i32], locals := [.i32], body := func43, results := [.i32] }
 
 def func44 : Wasm.Program :=
   [
@@ -5315,6 +5447,9 @@ def func44 : Wasm.Program :=
   .add,
   .globalSet 0
 ]
+
+def func44Def : Wasm.Function :=
+  { params := [.i32, .i32], locals := [.i32, .i32, .i64], body := func44, results := [] }
 
 def func45 : Wasm.Program :=
   [
@@ -5422,12 +5557,18 @@ def func45 : Wasm.Program :=
   .globalSet 0
 ]
 
+def func45Def : Wasm.Function :=
+  { params := [.i32, .i32], locals := [.i32, .i32, .i64], body := func45, results := [] }
+
 def func46 : Wasm.Program :=
   [
   .localGet 0,
   .const (0 : UInt32),
   .store32 (0 : UInt32)
 ]
+
+def func46Def : Wasm.Function :=
+  { params := [.i32, .i32], locals := [], body := func46, results := [] }
 
 def func47 : Wasm.Program :=
   [
@@ -5437,6 +5578,9 @@ def func47 : Wasm.Program :=
   .localGet 2,
   .call 54
 ]
+
+def func47Def : Wasm.Function :=
+  { params := [.i32, .i32, .i32], locals := [], body := func47, results := [.i32] }
 
 def func48 : Wasm.Program :=
   [
@@ -5496,6 +5640,9 @@ def func48 : Wasm.Program :=
   .store32 (0 : UInt32)
 ]
 
+def func48Def : Wasm.Function :=
+  { params := [.i32, .i32, .i32], locals := [.i32, .i32], body := func48, results := [] }
+
 def func49 : Wasm.Program :=
   [
   .block 0 0 [
@@ -5511,6 +5658,9 @@ def func49 : Wasm.Program :=
   .unreachable
 ]
 
+def func49Def : Wasm.Function :=
+  { params := [.i32, .i32], locals := [], body := func49, results := [] }
+
 def func50 : Wasm.Program :=
   [
   .localGet 1,
@@ -5518,6 +5668,9 @@ def func50 : Wasm.Program :=
   .call 31,
   .unreachable
 ]
+
+def func50Def : Wasm.Function :=
+  { params := [.i32, .i32], locals := [], body := func50, results := [] }
 
 def func51 : Wasm.Program :=
   [
@@ -5527,6 +5680,9 @@ def func51 : Wasm.Program :=
   .call 53,
   .unreachable
 ]
+
+def func51Def : Wasm.Function :=
+  { params := [], locals := [], body := func51, results := [] }
 
 def func52 : Wasm.Program :=
   [
@@ -5540,6 +5696,9 @@ def func52 : Wasm.Program :=
   .call 53,
   .unreachable
 ]
+
+def func52Def : Wasm.Function :=
+  { params := [.i32, .i32, .i32], locals := [], body := func52, results := [] }
 
 def func53 : Wasm.Program :=
   [
@@ -5572,6 +5731,9 @@ def func53 : Wasm.Program :=
   .call 30,
   .unreachable
 ]
+
+def func53Def : Wasm.Function :=
+  { params := [.i32, .i32, .i32], locals := [.i32], body := func53, results := [] }
 
 def func54 : Wasm.Program :=
   [
@@ -5881,6 +6043,9 @@ def func54 : Wasm.Program :=
   .localGet 5
 ]
 
+def func54Def : Wasm.Function :=
+  { params := [.i32, .i32, .i32, .i32], locals := [.i32, .i32, .i32, .i32, .i32, .i32, .i32, .i32], body := func54, results := [.i32] }
+
 def func55 : Wasm.Program :=
   [
   .globalGet 0,
@@ -5924,6 +6089,9 @@ def func55 : Wasm.Program :=
   .call 53,
   .unreachable
 ]
+
+def func55Def : Wasm.Function :=
+  { params := [.i32, .i32, .i32], locals := [.i32, .i64], body := func55, results := [] }
 
 def func56 : Wasm.Program :=
   [
@@ -6306,6 +6474,9 @@ def func56 : Wasm.Program :=
   ],
   .localGet 13
 ]
+
+def func56Def : Wasm.Function :=
+  { params := [.i32, .i32, .i32, .i32, .i32, .i32], locals := [.i32, .i32, .i32, .i32, .i32, .i32, .i32, .i32, .i64], body := func56, results := [.i32] }
 
 def func57 : Wasm.Program :=
   [
@@ -6810,6 +6981,9 @@ def func57 : Wasm.Program :=
   .localGet 8
 ]
 
+def func57Def : Wasm.Function :=
+  { params := [.i32, .i32], locals := [.i32, .i32, .i32, .i32, .i32, .i32, .i32, .i32], body := func57, results := [.i32] }
+
 def func58 : Wasm.Program :=
   [
   .block 0 0 [
@@ -6841,6 +7015,9 @@ def func58 : Wasm.Program :=
   .callIndirect 1 0
 ]
 
+def func58Def : Wasm.Function :=
+  { params := [.i32, .i32, .i32, .i32, .i32], locals := [], body := func58, results := [.i32] }
+
 def func59 : Wasm.Program :=
   [
   .localGet 0,
@@ -6852,6 +7029,9 @@ def func59 : Wasm.Program :=
   .load32 (12 : UInt32),
   .callIndirect 1 0
 ]
+
+def func59Def : Wasm.Function :=
+  { params := [.i32, .i32, .i32], locals := [], body := func59, results := [.i32] }
 
 def func60 : Wasm.Program :=
   [
@@ -7016,71 +7196,74 @@ def func60 : Wasm.Program :=
   .localGet 3
 ]
 
+def func60Def : Wasm.Function :=
+  { params := [.i32, .i32], locals := [.i32, .i32, .i32, .i32, .i32, .i32, .i32], body := func60, results := [.i32] }
+
 def «module» : Wasm.Module :=
 {
   imports := [],
   funcs := [
-    { params := [.i32, .i32], locals := [.i32, .i32, .i32, .i32], body := func0, results := [] },
-    { params := [.i32, .i32], locals := [.i32, .i32, .i32, .i32], body := func1, results := [] },
-    { params := [.i32, .i32], locals := [.i32, .i32, .i32, .i32], body := func2, results := [] },
-    { params := [.i32, .i32], locals := [], body := func3, results := [] },
-    { params := [.i32, .i32], locals := [], body := func4, results := [.i32] },
-    { params := [.i32, .i32, .i32], locals := [], body := func5, results := [] },
-    { params := [.i32, .i32, .i32, .i32], locals := [], body := func6, results := [.i32] },
-    { params := [], locals := [], body := func7, results := [] },
-    { params := [.i32, .i32], locals := [], body := func8, results := [.i32] },
-    { params := [.i32, .i32, .i32, .i32, .i32], locals := [.i32], body := func9, results := [] },
-    { params := [.i32, .i32], locals := [], body := func10, results := [] },
-    { params := [.i32], locals := [.i32], body := func11, results := [] },
-    { params := [.i32], locals := [.i32], body := func12, results := [] },
-    { params := [.i32], locals := [], body := func13, results := [] },
-    { params := [.i32], locals := [], body := func14, results := [] },
-    { params := [.i32], locals := [], body := func15, results := [] },
-    { params := [.i32], locals := [.i32, .i32, .i32], body := func16, results := [] },
-    { params := [.i32, .i32, .i32, .i32, .i32, .i32], locals := [.i32, .i32, .i64], body := func17, results := [] },
-    { params := [.i32, .i32, .i32, .i32, .i32], locals := [.i32, .i32], body := func18, results := [] },
-    { params := [.i32, .i32], locals := [], body := func19, results := [] },
-    { params := [.i32, .i32], locals := [], body := func20, results := [] },
-    { params := [.i32, .i32], locals := [], body := func21, results := [.i32] },
-    { params := [.i32, .i32], locals := [.i32, .i32, .i32, .i32, .i32], body := func22, results := [.i32] },
-    { params := [.i32], locals := [.i32, .i32, .i32, .i32, .i32, .i32, .i32, .i32, .i32, .i64], body := func23, results := [.i32] },
-    { params := [], locals := [], body := func24, results := [] },
-    { params := [.i32, .i32, .i32], locals := [.i32, .i32], body := func25, results := [] },
-    { params := [.i32], locals := [.i32, .i32, .i32, .i32], body := func26, results := [] },
-    { params := [.i32, .i32, .i32, .i32], locals := [.i32, .i32, .i32, .i32, .i32, .i32], body := func27, results := [.i32] },
-    { params := [.i32, .i32], locals := [.i32, .i32, .i32, .i32], body := func28, results := [] },
-    { params := [.i32, .i32], locals := [.i32, .i32], body := func29, results := [] },
-    { params := [.i32], locals := [.i32, .i64], body := func30, results := [] },
-    { params := [.i32, .i32], locals := [], body := func31, results := [] },
-    { params := [.i32, .i32], locals := [.i32], body := func32, results := [] },
-    { params := [.i32, .i32], locals := [.i32, .i32, .i32, .i32], body := func33, results := [] },
-    { params := [.i32], locals := [.i32, .i32], body := func34, results := [.i32] },
-    { params := [.i32, .i32], locals := [], body := func35, results := [] },
-    { params := [.i32, .i32], locals := [], body := func36, results := [] },
-    { params := [.i32, .i32], locals := [], body := func37, results := [.i32] },
-    { params := [.i32, .i32], locals := [], body := func38, results := [] },
-    { params := [.i32, .i32], locals := [], body := func39, results := [] },
-    { params := [.i32, .i32], locals := [.i32, .i32], body := func40, results := [] },
-    { params := [.i32, .i32], locals := [], body := func41, results := [.i32] },
-    { params := [.i32, .i32], locals := [.i32, .i32, .i32, .i32, .i32, .i32], body := func42, results := [.i32] },
-    { params := [.i32, .i32, .i32], locals := [.i32], body := func43, results := [.i32] },
-    { params := [.i32, .i32], locals := [.i32, .i32, .i64], body := func44, results := [] },
-    { params := [.i32, .i32], locals := [.i32, .i32, .i64], body := func45, results := [] },
-    { params := [.i32, .i32], locals := [], body := func46, results := [] },
-    { params := [.i32, .i32, .i32], locals := [], body := func47, results := [.i32] },
-    { params := [.i32, .i32, .i32], locals := [.i32, .i32], body := func48, results := [] },
-    { params := [.i32, .i32], locals := [], body := func49, results := [] },
-    { params := [.i32, .i32], locals := [], body := func50, results := [] },
-    { params := [], locals := [], body := func51, results := [] },
-    { params := [.i32, .i32, .i32], locals := [], body := func52, results := [] },
-    { params := [.i32, .i32, .i32], locals := [.i32], body := func53, results := [] },
-    { params := [.i32, .i32, .i32, .i32], locals := [.i32, .i32, .i32, .i32, .i32, .i32, .i32, .i32], body := func54, results := [.i32] },
-    { params := [.i32, .i32, .i32], locals := [.i32, .i64], body := func55, results := [] },
-    { params := [.i32, .i32, .i32, .i32, .i32, .i32], locals := [.i32, .i32, .i32, .i32, .i32, .i32, .i32, .i32, .i64], body := func56, results := [.i32] },
-    { params := [.i32, .i32], locals := [.i32, .i32, .i32, .i32, .i32, .i32, .i32, .i32], body := func57, results := [.i32] },
-    { params := [.i32, .i32, .i32, .i32, .i32], locals := [], body := func58, results := [.i32] },
-    { params := [.i32, .i32, .i32], locals := [], body := func59, results := [.i32] },
-    { params := [.i32, .i32], locals := [.i32, .i32, .i32, .i32, .i32, .i32, .i32], body := func60, results := [.i32] }
+    func0Def,
+    func1Def,
+    func2Def,
+    func3Def,
+    func4Def,
+    func5Def,
+    func6Def,
+    func7Def,
+    func8Def,
+    func9Def,
+    func10Def,
+    func11Def,
+    func12Def,
+    func13Def,
+    func14Def,
+    func15Def,
+    func16Def,
+    func17Def,
+    func18Def,
+    func19Def,
+    func20Def,
+    func21Def,
+    func22Def,
+    func23Def,
+    func24Def,
+    func25Def,
+    func26Def,
+    func27Def,
+    func28Def,
+    func29Def,
+    func30Def,
+    func31Def,
+    func32Def,
+    func33Def,
+    func34Def,
+    func35Def,
+    func36Def,
+    func37Def,
+    func38Def,
+    func39Def,
+    func40Def,
+    func41Def,
+    func42Def,
+    func43Def,
+    func44Def,
+    func45Def,
+    func46Def,
+    func47Def,
+    func48Def,
+    func49Def,
+    func50Def,
+    func51Def,
+    func52Def,
+    func53Def,
+    func54Def,
+    func55Def,
+    func56Def,
+    func57Def,
+    func58Def,
+    func59Def,
+    func60Def
   ],
   exports := [
     { name := "check", funcIdx := 3 }
