programs/lean/Project/XorSum/Program.lean
@@ -79,6 +79,9 @@ def func0 : Wasm.Program :=
   .unreachable
 ]
 
+def func0Def : Wasm.Function :=
+  { params := [.i32, .i32], locals := [.i32, .i32, .i32, .i32], body := func0, results := [] }
+
 def func1 : Wasm.Program :=
   [
   .const (0 : UInt32),
@@ -107,6 +110,9 @@ def func1 : Wasm.Program :=
   ],
   .localGet 2
 ]
+
+def func1Def : Wasm.Function :=
+  { params := [.i32, .i32], locals := [.i32], body := func1, results := [.i32] }
 
 def func2 : Wasm.Program :=
   [
@@ -149,6 +155,9 @@ def func2 : Wasm.Program :=
   .localGet 0
 ]
 
+def func2Def : Wasm.Function :=
+  { params := [.i32, .i32], locals := [.i32, .i32], body := func2, results := [.i32] }
+
 /-- export: check -/
 def func3 : Wasm.Program :=
   [
@@ -157,14 +166,17 @@ def func3 : Wasm.Program :=
   .call 0
 ]
 
+def func3Def : Wasm.Function :=
+  { params := [.i32, .i32], locals := [], body := func3, results := [] }
+
 def «module» : Wasm.Module :=
 {
   imports := [],
   funcs := [
-    { params := [.i32, .i32], locals := [.i32, .i32, .i32, .i32], body := func0, results := [] },
-    { params := [.i32, .i32], locals := [.i32], body := func1, results := [.i32] },
-    { params := [.i32, .i32], locals := [.i32, .i32], body := func2, results := [.i32] },
-    { params := [.i32, .i32], locals := [], body := func3, results := [] }
+    func0Def,
+    func1Def,
+    func2Def,
+    func3Def
   ],
   exports := [
     { name := "check", funcIdx := 3 }
