verifier/template/lean/Project/IsOdd/Proof.lean
@@ -8,6 +8,7 @@ open Wasm Project.IsOdd Project.IsOdd.Spec
 theorem is_odd_spec : IsOddSpec := by
   intro initial n
   wasm_entry
+  simp only [func0Def]
   unfold func0
   wp_run
   simp [UInt32.and_comm]
